ToyLanguageDef.fst
@@ -13,7 +13,7 @@ type lAExp =
   | LAExpMinus: lAExp  -> lAExp -> lAExp 
   | LAExpMult : lAExp  -> lAExp -> lAExp
   | LAExpDiv  : lAExp  -> lAExp -> lAExp
-  | LAExpCall : string -> list lAExp -> lAExp 
+  //| LAExpCall : string -> list lAExp -> lAExp 
 
 let ( +. ) = LAExpPlus
 let ( -. ) = LAExpMinus
@@ -41,13 +41,16 @@ instance _ : litteral_lift bool lBExp = { v = LBExpLitt }
 
 let ( !! ) = LAExpVar
 
+type lInstrAssignable = | AssignLAExp : lAExp -> lInstrAssignable
+                        | AssignCall  : string -> list lAExp -> lInstrAssignable
 
 type lInstr =
-  | LInstrAssign : string -> lAExp -> lInstr
+  | LInstrAssign : string -> lInstrAssignable -> lInstr
   | LInstrSkip   : lInstr
   | LInstrSeq    : lInstr -> lInstr -> lInstr
   | LInstrIf     : lBExp -> lInstr -> lInstr -> lInstr
   | LInstrWhile  : lBExp -> lInstr -> lInstr
+//  | LInstrStoCall: string -> string -> list lAExp -> lAExp 
   
 type funDef = | FunDef : string -> list string -> lInstr -> funDef
 
@@ -93,7 +96,7 @@ let rec lAExpToString exp = match exp with
          | LAExpMinus a b -> join " - " (L.map lAExpToString [a;b])
          | LAExpMult  a b -> join " * " (L.map lAExpToString [a;b])
          | LAExpDiv  a b  -> join " / " (L.map lAExpToString [a;b])
-         | LAExpCall name args -> name ^ "(" ^ (join ", " (L.map (admit (); lAExpToString) args)) ^ ")"
+         //| LAExpCall name args -> name ^ "(" ^ (join ", " (L.map (admit (); lAExpToString) args)) ^ ")"
          
 instance lAExpHasToString : hasToString lAExp = { toString = lAExpToString }
 let rec lBExpToString exp = match exp with
@@ -105,7 +108,11 @@ let rec lBExpToString exp = match exp with
   | LBExpLe  a b -> join " <= " (L.map toString [a;b])
 instance lBExpHasToString : hasToString lBExp = { toString = lBExpToString }
 let rec lInstrToString (n:nat) exp: Tot string (decreases exp) = match exp with
-  | LInstrAssign name v -> apptabs n (join " = " [name; toString v])
+  | LInstrAssign name v -> (match v with
+    | (AssignLAExp v) -> apptabs n (name ^ " = " ^ toString v)
+    | (AssignCall funName args) -> apptabs n (name ^ " = " ^ funName ^ "("
+                                  ^ join ", " (L.map toString args) ^ ")")
+    )
   | LInstrSkip -> apptabs n "SKIP"
   | LInstrSeq a b -> join "; \n" [lInstrToString n a; lInstrToString n b]
   | LInstrIf c a b -> join "" [apptabs n "if ("; toString c; ") {\n"; lInstrToString (n+1) a; "\n" `strcat` apptabs n "} else {\n"; lInstrToString (n+1) b; "\n" `strcat` apptabs n "}"]
@@ -115,12 +122,20 @@ instance lInstrHasToString : hasToString lInstr = { toString = lInstrToString 0 
 private
 let g t n (a: nat -> string)
   = let t' = t + 1 in ntabs t ^ n ^ " (\n" ^ a t' ^ "\n" ^ ntabs t ^ ")" 
+private
 let g' t n m (a: nat -> string)
   = let t' = t + 1 in ntabs t ^ n ^ " (" ^ m ^ " ,\n" ^ a t' ^ "\n" ^ ntabs t ^ ")" 
+private
 let h t n (a: nat -> string) (b: nat -> string)
   = let t' = t + 1 in ntabs t ^ n ^ " (\n" ^ a t' ^ ", \n" ^ b t' ^ "\n" ^ ntabs t ^ ")" 
+private
 let i t n (a: nat -> string) (b: nat -> string) (c: nat -> string)
   = let t' = t + 1 in ntabs t ^ n ^ " (\n" ^ a t' ^ ", \n" ^ b t' ^ ", \n" ^ c t' ^ "\n" ^ ntabs t ^ ")" 
+private
+let hh (t:nat) n (l: list (nat -> string))
+  = ntabs t ^ n ^ " (\n"
+    ^ join ", \n" (L.map (fun (f: nat -> string) -> f (t + 1)) l)
+    ^ "\n" ^ ntabs t ^ ")" 
 
 let rec print_AST_lAExp v (t: nat) = match v with
     | LAExpLitt n ->  ntabs t ^ toString n
@@ -129,7 +144,7 @@ let rec print_AST_lAExp v (t: nat) = match v with
     | LAExpMinus a b -> h t "LAExpMinus" (print_AST_lAExp a) (print_AST_lAExp b)
     | LAExpMult a b -> h t "LAExpMult" (print_AST_lAExp a) (print_AST_lAExp b)
     | LAExpDiv a b -> h t "LAExpDiv" (print_AST_lAExp a) (print_AST_lAExp b)
-    | LAExpCall name string -> "TODO"//h t "LAExpDiv" (print_AST_lAExp a) (print_AST_lAExp b)
+    //| LAExpCall name string -> "TODO"//h t "LAExpDiv" (print_AST_lAExp a) (print_AST_lAExp b)
 
 let rec print_AST_lBExp v (t: nat) = match v with
   | LBExpLitt n -> toString n
@@ -140,16 +155,38 @@ let rec print_AST_lBExp v (t: nat) = match v with
   | LBExpLe  a b -> h t "LBExpLe" (print_AST_lAExp a) (print_AST_lAExp b)  
 
 let rec print_AST_lInstr' v (t: nat) = match v with  
-  | LInstrAssign var value  -> g' t "LInstrAssign" var (print_AST_lAExp value)
+  | LInstrAssign var value  -> (match value with
+    | AssignLAExp value -> g' t "LInstrAssign.Exp" var (print_AST_lAExp value)
+    | AssignCall funName args -> hh t ("LInstrAssign.Call["^var^" <- "^funName^"(..)]") (L.map print_AST_lAExp args)
+    )
   | LInstrSkip              -> "LInstrSkip"
-  | LInstrSeq    a   b      -> h t "LInstrSeq" (print_AST_lInstr' a) (print_AST_lInstr' b)  
+  | LInstrSeq    a   b      -> 
+    let rec collect x = match x with | LInstrSeq a b -> collect a @ collect b
+                                     | _ -> [x] in
+    hh t "LInstrSeq" (L.map (admit();print_AST_lInstr') (collect v))
   | LInstrIf c btrue bfalse -> h t "LInstrIf" (print_AST_lBExp c) (print_AST_lInstr' btrue) 
   | LInstrWhile  c   body   -> h t "LInstrWhile" (print_AST_lBExp c) (print_AST_lInstr' body)
  
 let print_AST_lInstr v = print_AST_lInstr' v 0 
 
 
-let rec print_fullProg (funs, prog) t =
+let print_AST_fullProg (FullProg funs prog) = 
   let h = join "\n" in
-  [h (L.map (fun (FunDef name args body) -> "function " ^ name ^ " (" ^ join ", " args ^ ") {\n" ^ toString body ^ "\n}") funs), toString prog]
+  h [h (L.map 
+    (fun (FunDef name args body) -> "\n\n# Function " ^ name ^ " (" ^ join ", " args ^ "):\n"
+      ^ print_AST_lInstr body ^ "\n"
+    ) funs)
+  ; "\n\n # Main prog:" ^ print_AST_lInstr prog]
+
+private
+let rec print_tup_fullProg (FullProg funs prog): string =
+  let h = join "\n" in
+  h [h (L.map 
+    (fun (FunDef name args body) -> "function "
+       ^ name ^ " (" ^ join ", " args ^ ") {\n" ^ toString body ^ "\n}"
+    ) funs)
+  ; toString prog]
   
+instance fullProgHasToString : hasToString fullProg 
+         = { toString = print_tup_fullProg }
+
