ToyParser.fst
@@ -2,190 +2,18 @@ module ToyParser
 
 open FStar.String
 open FStar.Char
-module U32 = FStar.UInt32
 module L = FStar.List.Tot.Base
 open ToyLanguageDef
 
-module T = FStar.Tactics
+open ParserCombinators
+
 open ToString
-open MiscStuff
-module M = FStar.Mul
-
-let lowerCaseCharList = list_of_string "ABCDEFGHIJKLMNOPQRSTUVWXYZ"
-let upperCaseCharList = list_of_string "abcdefghijklmnopqrstuvwxyz"
-let digitList = list_of_string "1234567890"
-let isSpecialChar = list_of_string "~@#$%^?!+-*<>\\/|&=:"
-
-//type regexpSpecial = 
-
-type regexp a = | RegExpLit : a -> regexp a
-                | RegExpClassRange : (list a) -> regexp a
-                | RegExpAny : regexp a -> regexp a
-                | RegExpOr : regexp a -> regexp a -> regexp a
-                | RegExpSeq : regexp a -> regexp a -> regexp a
-                | RegExpEmpty : regexp a 
-
-type maybe a = | Nothing : maybe a | Just : a -> maybe a
-
-let op m1 m2 f1 f2 = match m1 with
-               | Just m1 -> (match m2 with
-                      | Just m2 -> Just (if f2 m1 m2 then f1 m1 else f1 m2)
-                      | Nothing -> Just (f1 m1))
-               | Nothing -> (match m2 with
-                      | Just m2 -> Just (f1 m2)
-                      | Nothing -> Nothing)
-
-let id x = x 
-
-// let bind x f = match x with | Nothing -> Nothing | Just v -> f v
 
 
-// let regexp_parse (#a:eqtype) (lst: list a) (re: regexp a) =
-//   let rec h (l acc: list a) (re: regexp a) : Tot (maybe (list a * list a)) (decreases re) = 
-//     let cmb left right = op (h l acc left) (h l acc right) id (fun (_,x) (_,y) -> L.length x < L.length y) in
-//     match l with
-//     | [] -> (match re with
-//            | RegExpLit _ -> Nothing
-//            | RegExpClassRange _ -> Nothing
-//            | RegExpAny _ -> Just (l, acc)
-//            | RegExpOr left right -> cmb left right
-//            | RegExpSeq e1 e2 -> r1 <-- h l acc e1; h (fst r1) (snd r1) e2 
-//            | RegExpEmpty -> Just (l, acc)
-//            )
-//     | hd::tl -> (match re with
-//            | RegExpLit a -> if a = hd then Just (tl, hd::acc) else Nothing
-//            | RegExpClassRange range -> if L.mem hd range then Just (tl, hd::acc) else Nothing
-//            | RegExpAny re' -> (match h l acc re' with
-//                              | Just (l', acc') -> h l' acc' re'
-//                              | Nothing -> Just (l, acc)
-//                              )
-//            | RegExpOr left right -> cmb left right
-//            | RegExpSeq e1 e2 -> r1 <-- h l acc e1; h (fst r1) (snd r1) e2
-//            | RegExpEmpty -> Just (l, acc)
-//            )
-//     in
-//   h lst [] re
-
-type parserResult a = | ParserRes : nat -> a -> parserResult a | NoRes
-
-type parser a = string -> nat -> parserResult a
-
-let empty #a (symb: a) : parser a = fun _ pos -> ParserRes pos symb
-let match_char #a (symb: a) (ch: char) : parser a = fun src pos -> if pos >= FStar.String.length src then NoRes
-                                                                else (
-                                                                  if get src pos = ch then ParserRes (pos+1) symb
-                                                                  else                     NoRes
-                                                                )
-                                                                
-let match_charf (f: char -> bool) : parser char = fun src pos -> if pos >= FStar.String.length src then NoRes
-                                                                else (let ch = get src pos in
-                                                                  if f ch then  ParserRes (pos+1) ch 
-                                                                  else    NoRes
-                                                                )
-
-type either a b = | Left : a -> either a b | Right : b -> either a b 
-
-let bind x f = match x with | ParserRes a b -> f (a, b) | _ -> NoRes
-
-let map_pr x f = x <-- x; ParserRes (fst x) (f (snd x))
-
-let fst' #a (x: parserResult a{ParserRes? x}) = match x with | ParserRes a _ -> a
-
-let comb_or #a #b #c (p_a: parser a) (p_b: parser b) (f: (either a b) -> c) : parser c = fun src pos -> 
-  let r_a = p_a src pos in
-  let r_b = p_b src pos in
-  match (r_a, r_b) with
-    | (NoRes, NoRes) -> NoRes
-    | (value, NoRes) -> map_pr value (f @ Left)
-    | (NoRes, value) -> map_pr value (f @ Right)
-    | (val0 , val1 ) -> if (fst' val0) > (fst' val1) then
-                            map_pr val0 (f @ Left)           
-                       else map_pr val1 (f @ Right)
-
-let rec repeat' #a (p_a: parser a) (acc:list a) src pos = 
-  match p_a src pos with
-    | ParserRes p v -> admitP (p << p); repeat' p_a (L.append acc [v]) src p
-    | NoRes -> ParserRes pos acc
-
-let repeat #a #b (p_a: parser a) (f: list a -> b) : parser b = fun src pos -> match repeat' p_a [] src pos with
-    | ParserRes p v -> ParserRes p (f v)
-    | NoRes -> NoRes
-
-let match_stringf (f: char -> bool) : parser string = repeat (match_charf f) string_of_list
-
-let sequence #a #b #c (p_a: parser a) (p_b: parser b) (f: a -> b -> c) : parser c = fun src pos ->
-  r_a <-- p_a src pos;
-  r_b <-- p_b src (fst r_a);
-  ParserRes (fst r_b) (f (snd r_a) (snd r_b))
-
-let match_string #a (str: string) (symb: a): parser a = fun src pos -> (L.fold_left (fun c char -> sequence c (match_char () char) (fun _ _ -> symb)) (empty symb) (list_of_string str)) src pos
-
-let (<*>) #t1 #t2 (a:parser t1) (b:parser t2): parser (t1*t2) = sequence a b (fun a b -> (a, b))
-let (<|>) = fun a b -> comb_or a b (fun e -> match e with | Left x -> x | Right x -> x)
-
-
-//let match_class #a (choices: list char) (symb: char -> a): parser a = fun src pos ->
-//  let p = (L.fold_left (fun c char -> comb_or c (match_char () char) (fun _ -> (Just char))) (empty Nothing) choices) src pos in
-//  match p with
-//  | ParserRes pos v -> (match v with | Just v -> ParserRes pos (symb v) | Nothing -> NoRes)
-//  | NoRes -> NoRes
-
-let match_class #a (choices: list char) (symb: char -> a): parser a = fun src pos ->
-  let p = L.fold_left (fun c char -> c <|> (match_char (Just char) char)) (empty Nothing) choices in
-  p <-- p src pos;
-  (match snd p with
-  | Just v -> ParserRes (fst p) (symb v)
-  | Nothing -> NoRes)
-
-let match_digit : parser (n: nat{n <= 9}) = 
-  let convert (c:char): (n: nat{n <= 9}) = match c with
-              | '1' -> 1 | '2' -> 2 | '3' -> 3 | '4' -> 4 | '5' -> 5
-              | '6' -> 6 | '7' -> 7 | '8' -> 8 | '9' -> 9 |  _  -> 0 in
-  match_class digitList convert
-
-let match_nat : parser nat =
-  let rec convert (c:list (n: nat{n <= 9})): nat = match c with
-    | [] -> 0
-    | hd::tl -> hd + (M.op_Star 10 (convert tl))
-  in
-  repeat match_digit (convert @ L.rev)
-
-let fp #a #b (f: a -> b) (p:parser a): parser b = fun src pos -> map_pr (p src pos) f
-
-let letterList = upperCaseCharList `L.append` lowerCaseCharList
-let match_word = repeat (match_class letterList id) string_of_list
-
+private
 let uncurry f x = let (l,r) = x in f l r
-
-let delayMe #a (p: unit -> parser a): parser a = fun a b -> (p ()) a b
-
-let (<*>>) a b = sequence a b (fun _ b -> b)
-let (<<*>) a b = sequence a b (fun a _ -> a)
-
-let match_space = match_class [' ';'\t';'\n';'\r'] (fun _ -> ())
-let any_space = repeat match_space (fun _ -> ())
-
-let match_eof: parser unit = fun src pos -> if pos >= String.length src then ParserRes pos () else NoRes 
-let match_eol: parser unit = match_char () '\n'
-
-let match_comment: parser string = any_space <*>> match_string "//" () <*>> match_stringf (fun x -> x <> '\n')
-
-let wrapspace #a (p: parser a): parser a = any_space <*>> p <<*> any_space 
-
-let opc ch: parser unit = wrapspace (match_char () ch)
-
+private
 let uncurry3 f x = let ((a,b),c) = x in f a b c
-
-let match_keyword str: parser unit = wrapspace (match_string str ())
-let match_kwds (strs:list string{L.length strs > 0}): parser unit = 
-  let hd::tl = strs in
-    L.fold_left (fun c kw -> c <*>> match_keyword kw) (match_keyword hd) tl 
-
-let match_maybe #a (p:parser a): parser (maybe a) = fun src pos -> match p src pos with
-                | ParserRes x y -> ParserRes x (Just y)
-                | NoRes -> ParserRes pos Nothing
-
-let match_comments: parser (maybe (list string)) = match_maybe (repeat match_comment (fun l -> l))
 
 let aexp_parser: parser lAExp =
   let rec no_rec (): parser lAExp = fp LAExpLitt match_nat <|> fp LAExpVar match_word
@@ -197,10 +25,8 @@ let aexp_parser: parser lAExp =
                    <|> fp (uncurry LAExpDiv)  (no_rec () <<*> opc '/' <*> h)
   in wrapspace (h' ())
 
-let bool_litt_parser: parser bool = any_space <*>> match_string "true" true <|> match_string "false" false <<*> any_space
-
 let bexp_parser: parser lBExp =
-  let rec no_rec (): parser lBExp = fp LBExpLitt bool_litt_parser
+  let rec no_rec (): parser lBExp = fp LBExpLitt match_boolean_litterate
            <|> fp (uncurry LBExpEq) (aexp_parser <<*> match_string "==" () <*> aexp_parser)
            <|> fp (uncurry LBExpLe) (aexp_parser <<*> match_string "<=" () <*> aexp_parser)
            <|> fp LBExpNot (match_char () '~' <*>> (admitP (() << ()); delayMe no_rec))
@@ -213,7 +39,7 @@ let bexp_parser: parser lBExp =
 
 private
 type lFakeInstr =
-  | LFakeInstrAssign : string -> lAExp -> lFakeInstr
+  | LFakeInstrAssign : string -> lInstrAssignable -> lFakeInstr
   | LFakeInstrSkip   : lFakeInstr
   | LFakeInstrSeq    : lFakeInstr -> lFakeInstr -> lFakeInstr
   | LFakeInstrIf     : lBExp -> lFakeInstr -> lFakeInstr -> lFakeInstr
@@ -222,8 +48,12 @@ type lFakeInstr =
 and funFakeDef = | FunFakeDef : string -> list string -> lFakeInstr -> funFakeDef
 
 
-private
-let args_parser: parser (list string) = wrapspace (match_keyword "(" <*>> (repeat match_word id) <<*> match_keyword ")")
+
+instance pr_ts #a [| hasToString a |] : hasToString (parserResult a) = { 
+   toString = fun v -> match v with
+    | ParserRes pos somevalue -> join "" ["{pos:"; string_of_int pos ; "} "; toString somevalue]
+    | NoRes -> "NoRes"
+}
 
 private
 let rec lFakeInstrIsWF prog toplevel = match prog with 
@@ -236,29 +66,32 @@ private
 type lFakeInstrWF = r:lFakeInstr {lFakeInstrIsWF r true}
 
 private
-let parseFun (p: parser lFakeInstr): parser ((string * list string) * lFakeInstr) = (
-                  (match_keyword "function" <*>> match_word <*> args_parser <<*> match_keyword "{")
-              <*> (p <<*> match_keyword "}")
-           )
+let hAssignCall var fName args = LFakeInstrAssign var (AssignCall fName args)
+private
+let hAssignExp var exp = LFakeInstrAssign var (AssignLAExp exp) 
 
 private
 let lFakeInstr_parser: parser (r:lFakeInstr {lFakeInstrIsWF r true}) =
    let z #a (arg:parser a) = arg <<*> match_comments in
    let rec no_rec (tl:bool): parser (r:lFakeInstr {lFakeInstrIsWF r tl}) = admitP (() << ()); z (
-           fp (uncurry LFakeInstrAssign) (match_word <<*> match_keyword "=" <*> aexp_parser)
+           fp (uncurry hAssignExp) (match_word <<*> match_keyword "=" <*> aexp_parser)
+       <|> fp (uncurry3 hAssignCall) (match_word <<*> match_keyword "="
+              <*> match_word <*> match_list "(" ")" aexp_parser)
        <|> match_string "SKIP" LFakeInstrSkip
        <|> fp (uncurry3 LFakeInstrIf) (
-                  ((match_kwds ["if"; "("] <*>> bexp_parser) <<*> match_kwds [")"; "{"])
-              <*> ((delayMe (h' false)) <<*> match_kwds ["}";"else";"{"])
+                  ((match_keywords ["if"; "("] <*>> bexp_parser) <<*> match_keywords [")"; "{"])
+              <*> ((delayMe (h' false)) <<*> match_keywords ["}";"else";"{"])
               <*> ((delayMe (h' false)) <<*> match_keyword "}")
            )
        <|> fp (fun ((str,args),body) -> LFakeInstrFunDef (FunFakeDef str args body)) (
-                  (match_keyword "function" <*>> match_word <*> args_parser <<*> match_keyword "{")
+                  (match_keyword "function" <*>> match_word <*> 
+                    (match_list "(" ")" match_word)
+                    <<*> match_keyword "{")
               <*> (delayMe (h' false) <<*> match_keyword "}")
            )       
        <|> fp (uncurry LFakeInstrWhile) (
-                  ((match_kwds ["while";"("] <*>> bexp_parser) <<*> match_kwds [")";"{"])
-              <*> ((delayMe (h' true)) <<*> match_keyword "}")
+                  ((match_keywords ["while";"("] <*>> bexp_parser) <<*> match_keywords [")";"{"])
+              <*> ((delayMe (h' false)) <<*> match_keyword "}")
            ))
    and h' (tl:bool) (): parser (r:lFakeInstr {lFakeInstrIsWF r tl}) = admitP (() << ()); let h = delayMe (h' tl) in
      z (
@@ -285,31 +118,11 @@ let wfFakeConv (r:lFakeInstr {lFakeInstrIsWF r true}): (list funDef * lInstr) =
   | LFakeInstrFunDef (FunFakeDef name args body) -> ([FunDef name args (let (_,b) = h false body in b)], LInstrSkip)
   ) in h true r
   
-let lInstr_parser: parser fullProg =
+let fullProg_parser: parser fullProg =
   fp (fun x -> let (a, b) = wfFakeConv x in FullProg a b) lFakeInstr_parser
 
-instance pr_ts #a [| hasToString a |] : hasToString (parserResult a) = { 
-   toString = fun v -> match v with
-    | ParserRes pos somevalue -> join "" ["{pos:"; string_of_int pos ; "} "; toString somevalue]
-    | NoRes -> "NoRes"
-}
 
-let parse_toy_language src = match (lInstr_parser <<*> match_eof) src 0 with
-  | ParserRes _ res -> Just res
-  | NoRes -> Nothing
-  
-//let ttt = lFakeInstr_parser//match_class ['a';'b'] id //(match_char "GOT A" 'a') <|> (match_char "GOT B" 'b')
+let parse_toy_language src = match (fullProg_parser <<*> match_eof) src 0 with
+  | ParserRes _ res -> Some res
+  | NoRes -> None
 
-//let sss = ttt ()
-
-//let xxx = String.strcat (pr_ts.toString (ttt "if     (6+54+hey<=8) {a=3} else {b=2}" 0)) "\n"
-//let xxx s = String.strcat (pr_ts.toString (ttt s 0)) "\n"
-
-//let _ = assert (xxx = magic ()) by (T.compute (); T.qed ())
-
-// let lexer (input: string) =
-//   let h (list:list char) = match list with
-//     []    -> []
-//     hd::tl -> (match hd with
-//       'a' -> )
-  
