README.md
@@ -7,3 +7,5 @@ Brief description of main modules
  - [AbstractDomain](AbstractDomain.fst): defines a what an abstract domain is
  - [StaticAnalyser](StaticAnalyser.fst): core of the analyser
  - [CSet](CSet.fst): enumerable non-ordered sets
+
+## Compiling to native
